more proof work

lib/Base/Multisets.i.dfy
@@ -1,3 +1,5 @@
+include "Maps.s.dfy"
+
 module Multisets {
   function {:opaque} Choose<A>(s: multiset<A>) : (result: A)
     requires 0 < |s|
@@ -73,54 +75,106 @@ module Multisets {
       }
     }
   }
+
+  predicate Foldable<A(!new)>(zero: A, add: (A, A) ~> A, inv: A -> bool)
+    reads set x, y, o | inv(x) && inv(y) && o in add.reads(x, y) :: o
+  {
+    && inv(zero)
+    && forall x, y | inv(x) && inv(y) :: add.requires(x, y) && inv(add(x, y))
+  }
   
-  function {:opaque} Fold<A>(zero: A, add: (A, A) -> A, s: multiset<A>) : (result: A)
+  function {:opaque} Fold<A(!new)>(zero: A, add: (A, A) ~> A, inv: A -> bool, s: multiset<A>) : (result: A)
+    requires Foldable(zero, add, inv)
+    requires forall x | x in s :: inv(x)
     ensures |s| == 0 ==> result == zero
+    ensures inv(result)
+    reads set x, y, o | inv(x) && inv(y) && o in add.reads(x, y) :: o
   {
     if |s| == 0 then
       zero
     else
       var a := Choose(s);
-      add(a, Fold(zero, add, s - multiset{a}))
+      add(a, Fold(zero, add, inv, s - multiset{a}))
   }
 
-  lemma FoldSingleton<A>(zero: A, add: (A, A) -> A, x: A)
-    ensures Fold(zero, add, multiset{x}) == add(x, zero)
+  function FoldSimple<A>(zero: A, add: (A, A) -> A, s: multiset<A>) : (result: A)
+    ensures |s| == 0 ==> result == zero
+  {
+    Fold(zero, add, x => true, s)
+  }
+
+  lemma FoldSingleton<A>(zero: A, add: (A, A) ~> A, inv: A -> bool, x: A)
+    requires Foldable(zero, add, inv)
+    requires inv(x)
+    ensures Fold(zero, add, inv, multiset{x}) == add(x, zero)
   {
     reveal_Fold();
   }
   
-  predicate {:opaque} IsIdentity<A(!new)>(add: (A, A) -> A, zero: A) {
-    && forall a :: add(zero, a) == add(a, zero) == a
+  lemma FoldSimpleSingleton<A>(zero: A, add: (A, A) -> A, x: A)
+    ensures FoldSimple(zero, add, multiset{x}) == add(x, zero)
+  {
+    reveal_Fold();
+  }
+  
+  predicate {:opaque} IsIdentity<A(!new)>(add: (A, A) ~> A, inv: A -> bool, zero: A)
+    reads set x, y, o | inv(x) && inv(y) && o in add.reads(x, y) :: o
+  {
+    && Foldable(zero, add, inv)
+    && forall a | inv(a) :: add(zero, a) == add(a, zero) == a
   }
 
-  predicate {:opaque} IsCommutative<A(!new)>(add: (A, A) -> A) {
-    forall a, b :: add(a, b) == add(b, a)
+  predicate {:opaque} IsCommutative<A(!new)>(add: (A, A) ~> A, inv: A -> bool)
+    requires forall x, y | inv(x) && inv(y) :: add.requires(x, y)
+    reads set x, y, o | inv(x) && inv(y) && o in add.reads(x, y) :: o
+  {
+    forall a, b | inv(a) && inv(b) :: add(a, b) == add(b, a)
   }
 
-  predicate {:opaque} IsAssociative<A(!new)>(add: (A, A) -> A) {
-    forall a, b, c :: add(add(a, b), c) == add(a, add(b, c))
+  predicate {:opaque} IsAssociative<A(!new)>(add: (A, A) ~> A, inv: A -> bool)
+    requires forall x, y | inv(x) && inv(y) :: add.requires(x, y) && inv(add(x, y))
+    reads set x, y, o | inv(x) && inv(y) && o in add.reads(x, y) :: o
+  {
+    forall a, b, c | inv(a) && inv(b) && inv(c) :: add(add(a, b), c) == add(a, add(b, c))
   }
 
-  lemma FoldAdditive<A>(zero: A, add: (A, A) -> A, s1: multiset<A>, s2: multiset<A>)
-    requires IsCommutative(add)
-    requires IsAssociative(add)
-    requires IsIdentity(add, zero)
-    ensures Fold(zero, add, s1 + s2) == add(Fold(zero, add, s1), Fold(zero, add, s2))
+  
+  predicate IsIdentitySimple<A(!new)>(add: (A, A) -> A, zero: A)
+  {
+    IsIdentity(add, x => true, zero)
+  }
+
+  predicate IsCommutativeSimple<A(!new)>(add: (A, A) -> A)
+  {
+    IsCommutative(add, x => true)
+  }
+
+  predicate IsAssociativeSimple<A(!new)>(add: (A, A) -> A) {
+    IsAssociative(add, x => true)
+  }
+
+  lemma FoldAdditive<A>(zero: A, add: (A, A) ~> A, inv: A -> bool, s1: multiset<A>, s2: multiset<A>)
+    requires Foldable(zero, add, inv)
+    requires forall x | x in s1 :: inv(x)
+    requires forall x | x in s2 :: inv(x)
+    requires IsCommutative(add, inv)
+    requires IsAssociative(add, inv)
+    requires IsIdentity(add, inv, zero)
+    ensures Fold(zero, add, inv, s1 + s2) == add(Fold(zero, add, inv, s1), Fold(zero, add, inv, s2))
     decreases |s1| + |s2|
   {
-    var f1 := Fold(zero, add, s1);
-    var f2 := Fold(zero, add, s2);
-    var fs := Fold(zero, add, s1 + s2);
+    var f1 := Fold(zero, add, inv, s1);
+    var f2 := Fold(zero, add, inv, s2);
+    var fs := Fold(zero, add, inv, s1 + s2);
     if |s1| == 0 {
       assert s1 + s2 == s2;
-      assert add(f1, f2) == Fold(zero, add, s2) by {
+      assert add(f1, f2) == Fold(zero, add, inv, s2) by {
         reveal_IsIdentity();
         reveal_Fold();
       }
     } else if |s2| == 0 {
       assert s1 + s2 == s1;
-      assert add(f1, f2) == Fold(zero, add, s1) by {
+      assert add(f1, f2) == Fold(zero, add, inv, s1) by {
         reveal_IsIdentity();
         reveal_Fold();
       }
@@ -131,43 +185,60 @@ module Multisets {
         calc {
           fs;
           { reveal_Fold(); }
-          add(x, Fold(zero, add, (s1 + s2) - multiset{x}));
+          add(x, Fold(zero, add, inv, (s1 + s2) - multiset{x}));
           { assert (s1 + s2) - multiset{x} == (s1 - multiset{x}) + s2; }
-          add(x, Fold(zero, add, (s1 - multiset{x}) + s2));
-          { FoldAdditive(zero, add, s1 - multiset{x}, s2); }
-          add(x, add(Fold(zero, add, s1 - multiset{x}), Fold(zero, add, s2)));
+          add(x, Fold(zero, add, inv, (s1 - multiset{x}) + s2));
+          { FoldAdditive(zero, add, inv, s1 - multiset{x}, s2); }
+          add(x, add(Fold(zero, add, inv, s1 - multiset{x}), Fold(zero, add, inv, s2)));
           { reveal_IsAssociative(); }
-          add(add(x, Fold(zero, add, s1 - multiset{x})), Fold(zero, add, s2));
+          add(add(x, Fold(zero, add, inv, s1 - multiset{x})), Fold(zero, add, inv, s2));
           { reveal_IsIdentity(); reveal_Fold(); }
-          add(add(Fold(zero, add, multiset{x}), Fold(zero, add, s1 - multiset{x})), Fold(zero, add, s2));
-          { FoldAdditive(zero, add, multiset{x}, s1 - multiset{x}); }
-          add(Fold(zero, add, multiset{x} + (s1 - multiset{x})), Fold(zero, add, s2));
+          add(add(Fold(zero, add, inv, multiset{x}), Fold(zero, add, inv, s1 - multiset{x})), Fold(zero, add, inv, s2));
+          { FoldAdditive(zero, add, inv, multiset{x}, s1 - multiset{x}); }
+          add(Fold(zero, add, inv, multiset{x} + (s1 - multiset{x})), Fold(zero, add, inv, s2));
           { assert multiset{x} + (s1 - multiset{x}) == s1; }
-          add(Fold(zero, add, s1), Fold(zero, add, s2));
+          add(Fold(zero, add, inv, s1), Fold(zero, add, inv, s2));
         }
       } else {
         calc {
           fs;
           { reveal_Fold(); }
-          add(x, Fold(zero, add, (s1 + s2) - multiset{x}));
+          add(x, Fold(zero, add, inv, (s1 + s2) - multiset{x}));
           { assert (s1 + s2) - multiset{x} == s1 + (s2 - multiset{x}); }
-          add(x, Fold(zero, add, s1 + (s2 - multiset{x})));
-          { FoldAdditive(zero, add, s1, s2 - multiset{x}); }
-          add(x, add(Fold(zero, add, s1), Fold(zero, add, s2 - multiset{x})));
+          add(x, Fold(zero, add, inv, s1 + (s2 - multiset{x})));
+          { FoldAdditive(zero, add, inv, s1, s2 - multiset{x}); }
+          add(x, add(Fold(zero, add, inv, s1), Fold(zero, add, inv, s2 - multiset{x})));
           { reveal_IsAssociative(); }
-          add(add(x, Fold(zero, add, s1)), Fold(zero, add, s2 - multiset{x}));
+          add(add(x, Fold(zero, add, inv, s1)), Fold(zero, add, inv, s2 - multiset{x}));
           { reveal_IsCommutative(); }
-          add(add(Fold(zero, add, s1), x), Fold(zero, add, s2 - multiset{x}));
+          add(add(Fold(zero, add, inv, s1), x), Fold(zero, add, inv, s2 - multiset{x}));
           { reveal_IsAssociative(); }
-          add(Fold(zero, add, s1), add(x, Fold(zero, add, s2 - multiset{x})));
+          add(Fold(zero, add, inv, s1), add(x, Fold(zero, add, inv, s2 - multiset{x})));
           { reveal_IsIdentity(); reveal_Fold(); }
-          add(Fold(zero, add, s1), add(Fold(zero, add, multiset{x}), Fold(zero, add, s2 - multiset{x})));
-          { FoldAdditive(zero, add, multiset{x}, s2 - multiset{x}); }
-          add(Fold(zero, add, s1), Fold(zero, add, multiset{x} + (s2 - multiset{x})));
-          assert multiset{x} + (s2 - multiset{x}) == s2;
-          add(Fold(zero, add, s1), Fold(zero, add, s2));
+          add(Fold(zero, add, inv, s1), add(Fold(zero, add, inv, multiset{x}), Fold(zero, add, inv, s2 - multiset{x})));
+          { FoldAdditive(zero, add, inv, multiset{x}, s2 - multiset{x}); }
+          add(Fold(zero, add, inv, s1), Fold(zero, add, inv, multiset{x} + (s2 - multiset{x})));
+          { assert multiset{x} + (s2 - multiset{x}) == s2; }
+          add(Fold(zero, add, inv, s1), Fold(zero, add, inv, s2));
         }
       }
     }
+  }
+
+  lemma FoldSimpleAdditive<A>(zero: A, add: (A, A) -> A, s1: multiset<A>, s2: multiset<A>)
+    requires IsCommutativeSimple(add)
+    requires IsAssociativeSimple(add)
+    requires IsIdentitySimple(add, zero)
+    ensures FoldSimple(zero, add, s1 + s2) == add(FoldSimple(zero, add, s1), FoldSimple(zero, add, s2))
+  {
+    FoldAdditive(zero, add, x => true, s1, s2);
+  }  
+
+  // TODO(rob): not really the right place for this, but can't put it
+  // in Maps, since that's trusted, which precludes including this
+  // file in Maps.s.dfy.
+  function ValueMultiset<A,B>(m: map<A,B>) : (result: multiset<B>)
+  {
+    Apply(x requires x in m => m[x], multiset(m.Keys))
   }
 }
